Cache.v: clean up proofs and implement validator-based replacement algorithm
The cache now invokes an external replacement algorithm to keep track
of what blocks are being accessed, and to choose a block when evicting.
If the replacement algorithm malfunctions, and returns a block that is not
in the cache, the cache code will choose its own block to evict instead.

Amusingly, because of Haskell's lazy evaluation, even though every
disk access is supposed to update the replacement algorithm state, it
never gets evaluated (because we never evict in our workloads), so the
fact that there is no actual implementation doesn't bother Haskell --
the file system continues to work!  I expect it will throw an exception
when it needs to actually evict some block, and then we can implement
some replacement algorithm.

Also add a paragraph to the paper about this validating replacement
approach.

A few admits left about lengths of [Map.cardinal].  I decided to use [nat]
instead of [word] for keeping track of the current cache size.  Since this
value is not exported to/from disk, there's no reason to keep it as
[word].  Avoiding [word] made the proofs much easier and much faster.

src/Cache.v
@@ -16,28 +16,43 @@ Module Map := FMapAVL.Make(Addr_as_OT).
 Import ListNotations.
 Set Implicit Arguments.
 
+Parameter eviction_state : Type.
+Parameter eviction_init : eviction_state.
+Parameter eviction_update : eviction_state -> addr -> eviction_state.
+Parameter eviction_choose : eviction_state -> (addr * eviction_state).
+
 Record cachestate := {
   CSMap : Map.t valu;
-  CSCount : addr;  (* current number of items, for efficient capacity checks *)
-  CSMaxCount : addr
+  CSCount : nat;
+  CSMaxCount : nat;
+  CSEvict : eviction_state
 }.
 
 Module BUFCACHE.
 
   Definition rep (cs : cachestate) (m : @mem addr (@weq addrlen) valuset) :=
     (diskIs m *
-     [[ Map.cardinal (CSMap cs) = # (CSCount cs) ]] *
-     [[ (CSCount cs <= CSMaxCount cs)%word ]] *
-     [[ CSMaxCount cs <> $0 ]] *
+     [[ Map.cardinal (CSMap cs) = CSCount cs ]] *
+     [[ CSCount cs <= CSMaxCount cs ]] *
+     [[ CSMaxCount cs <> 0 ]] *
      [[ forall a v, Map.MapsTo a v (CSMap cs) -> exists old, m a = Some (v, old) ]])%pred.
 
   Definition trim T (cs : cachestate) rx : prog T :=
-    If (wlt_dec (CSCount cs) (CSMaxCount cs)) {
+    If (lt_dec (CSCount cs) (CSMaxCount cs)) {
       rx cs
     } else {
-      match (Map.elements (CSMap cs)) with
-      | nil => rx cs
-      | (a,v) :: tl => rx (Build_cachestate (Map.remove a (CSMap cs)) (CSCount cs ^- $1) (CSMaxCount cs))
+      let (victim, evictor) := eviction_choose (CSEvict cs) in
+      match (Map.find victim (CSMap cs)) with
+      | Some v => rx (Build_cachestate (Map.remove victim (CSMap cs))
+                                       (CSCount cs - 1)
+                                       (CSMaxCount cs) evictor)
+      | None => (* evictor failed, evict first block *)
+        match (Map.elements (CSMap cs)) with
+        | nil => rx cs
+        | (a,v) :: tl => rx (Build_cachestate (Map.remove a (CSMap cs))
+                                              (CSCount cs - 1)
+                                              (CSMaxCount cs) (CSEvict cs))
+        end
       end
     }.
 
@@ -47,7 +62,8 @@ Module BUFCACHE.
     | Some v => rx (cs, v)
     | None =>
       v <- Read a;
-      rx (Build_cachestate (Map.add a v (CSMap cs)) (CSCount cs ^+ $1) (CSMaxCount cs), v)
+      rx (Build_cachestate (Map.add a v (CSMap cs)) (CSCount cs + 1)
+                           (CSMaxCount cs) (eviction_update (CSEvict cs) a), v)
     end.
 
   Definition write T a v (cs : cachestate) rx : prog T :=
@@ -55,21 +71,19 @@ Module BUFCACHE.
     Write a v;;
     match Map.find a (CSMap cs) with
     | Some _ =>
-      rx (Build_cachestate (Map.add a v (CSMap cs)) (CSCount cs) (CSMaxCount cs))
+      rx (Build_cachestate (Map.add a v (CSMap cs)) (CSCount cs)
+                           (CSMaxCount cs) (eviction_update (CSEvict cs) a))
     | None =>
-      rx (Build_cachestate (Map.add a v (CSMap cs)) (CSCount cs ^+ $1) (CSMaxCount cs))
+      rx (Build_cachestate (Map.add a v (CSMap cs)) (CSCount cs + 1)
+                           (CSMaxCount cs) (eviction_update (CSEvict cs) a))
     end.
 
   Definition sync T a (cs : cachestate) rx : prog T :=
     Sync a;;
     rx cs.
 
-  Definition init T (cachesize : addr) (rx : cachestate -> prog T) : prog T :=
-    If (weq cachesize $0) {
-      rx (Build_cachestate (Map.empty valu) $0 $1)
-    } else {
-      rx (Build_cachestate (Map.empty valu) $0 cachesize)
-    }.
+  Definition init T (cachesize : nat) (rx : cachestate -> prog T) : prog T :=
+    rx (Build_cachestate (Map.empty valu) 0 cachesize eviction_init).
 
   Definition read_array T a i cs rx : prog T :=
     r <- read (a ^+ i ^* $1) cs;
@@ -92,14 +106,28 @@ Module BUFCACHE.
     congruence.
   Qed.
 
-  Lemma map_remove_cardinal : forall V (m : Map.t V) k, Map.In k m ->
+  Lemma map_remove_cardinal : forall (m : Map.t valu) k, (exists v, Map.MapsTo k v m) ->
     Map.cardinal (Map.remove k m) = Map.cardinal m - 1.
+  Proof.
+    admit.
+(*
+    intros.
+    repeat rewrite Map.cardinal_1.
+    erewrite filter_split with (l:=Map.elements m);
+      try apply Map.elements_3.
+    instantiate (f := fun e => if weq k (fst e) then true else false).
+    rewrite app_length.
+*)
+  Qed.
+
+  Lemma map_add_cardinal : forall V (m : Map.t V) k v, ~ (exists v, Map.MapsTo k v m) ->
+    Map.cardinal (Map.add k v m) = Map.cardinal m + 1.
   Proof.
     admit.
   Qed.
 
-  Lemma map_add_cardinal : forall V (m : Map.t V) k v, ~ Map.In k m ->
-    Map.cardinal (Map.add k v m) = Map.cardinal m + 1.
+  Lemma map_add_dup_cardinal : forall V (m : Map.t V) k v, (exists v, Map.MapsTo k v m) ->
+    Map.cardinal (Map.add k v m) = Map.cardinal m.
   Proof.
     admit.
   Qed.
@@ -117,6 +145,7 @@ Module BUFCACHE.
 
   Hint Resolve Map.remove_3.
   Hint Resolve Map.add_3.
+  Hint Resolve Map.find_2.
   Hint Resolve mapsto_add.
 
   Ltac unfold_rep := unfold rep.
@@ -124,30 +153,24 @@ Module BUFCACHE.
   Theorem trim_ok : forall cs,
     {< d,
     PRE      rep cs d
-    POST:cs' rep cs' d
+    POST:cs  rep cs d *
+             [[ CSCount cs < CSMaxCount cs ]]
     CRASH    exists cs', rep cs' d
     >} trim cs.
   Proof.
     unfold trim, rep; hoare.
-    destruct cs as [cmap cnum].
-    case_eq (Map.elements cmap); hoare.
+    destruct (eviction_choose (CSEvict cs)).
 
-    rewrite map_remove_cardinal by (eapply map_elements_hd_in; eauto).
-    rewrite H6.
-    destruct xp; simpl in *.
+    case_eq (Map.find w (CSMap cs)); hoare.
+    rewrite map_remove_cardinal; eauto.
 
-    rewrite wminus_Alt. rewrite wminus_Alt2. unfold wordBinN.
-    erewrite wordToNat_natToWord_bound with (bound:=cnum).
-    reflexivity.
-    omega.
-    intro; apply H8; clear H8.
-    apply lt_wlt.
-    apply wlt_lt in H0.
-    simpl in *.
-    case_eq (#MaxCacheBlocks0); intros; try omega.
-    rewrite <- H1 in MaxCacheBlocksOK0.
-    rewrite natToWord_wordToNat in MaxCacheBlocksOK0.
-    congruence.
+    case_eq (Map.elements (CSMap cs)); hoare.
+    replace (CSCount cs) with (CSMaxCount cs) in * by omega.
+    rewrite Map.cardinal_1 in *. rewrite H in *; clear H.
+    simpl in *; omega.
+
+    destruct p0; hoare.
+    rewrite map_remove_cardinal by (eapply map_elements_hd_in; eauto); eauto.
   Qed.
 
   Hint Extern 1 ({{_}} progseq (trim _) _) => apply trim_ok : prog.
@@ -155,26 +178,26 @@ Module BUFCACHE.
   Theorem read_ok : forall cs a,
     {< d F v,
     PRE          rep cs d * [[ (F * a |~> v)%pred d ]]
-    POST:(cs',r) rep cs' d * [[ r = v ]]
+    POST:(cs,r)  rep cs d * [[ r = v ]]
     CRASH        exists cs', rep cs' d
     >} read a cs.
   Proof.
     unfold read.
     hoare_unfold unfold_rep.
 
-    apply sep_star_comm in H3.
-    apply ptsto_valid in H3 as H'.
-    destruct (Map.find a (fst r_)) eqn:Hfind; hoare.
+    apply ptsto_valid' in H3 as H'.
+    destruct (Map.find a (CSMap r_)) eqn:Hfind; hoare.
 
-    apply Map.find_2 in Hfind. apply H9 in Hfind. rewrite H' in Hfind. deex; congruence.
+    apply Map.find_2 in Hfind. apply H12 in Hfind. rewrite H' in Hfind. deex; congruence.
     rewrite diskIs_extract with (a:=a); try pred_apply; cancel.
     rewrite <- diskIs_combine_same with (m:=m); try pred_apply; cancel.
 
-    admit.
+    rewrite map_add_cardinal; auto.
+    intro Hm; destruct Hm as [? Hm]. apply Map.find_1 in Hm. congruence.
 
     destruct (weq a a0); subst.
     apply mapsto_add in H; subst; eauto.
-    edestruct H9. eauto. eexists; eauto.
+    edestruct H12. eauto. eexists; eauto.
 
     rewrite <- diskIs_combine_same with (m:=m); try pred_apply; cancel.
   Qed.
@@ -184,8 +207,8 @@ Module BUFCACHE.
   Theorem write_ok : forall cs a v,
     {< d F v0,
     PRE      rep cs d * [[ (F * a |-> v0)%pred d ]]
-    POST:cs' exists d',
-             rep cs' d' * [[ (F * a |-> (v, valuset_list v0))%pred d' ]]
+    POST:cs  exists d',
+             rep cs d' * [[ (F * a |-> (v, valuset_list v0))%pred d' ]]
     CRASH    exists cs', rep cs' d \/
              exists d', rep cs' d' * [[ (F * a |-> (v, valuset_list v0))%pred d' ]]
     >} write a v cs.
@@ -194,10 +217,10 @@ Module BUFCACHE.
     hoare_unfold unfold_rep.
 
     rewrite diskIs_extract with (a:=a); try pred_apply; cancel.
-    destruct (Map.find a (fst r_)); hoare.
+    destruct (Map.find a (CSMap r_)) eqn:Hfind; hoare.
 
     rewrite <- diskIs_combine_upd with (m:=m); try pred_apply; cancel.
-    admit.
+    rewrite map_add_dup_cardinal; eauto.
     destruct (weq a a0); subst.
     apply mapsto_add in H; subst.
     rewrite upd_eq by auto. eauto.
@@ -208,7 +231,8 @@ Module BUFCACHE.
     eapply ptsto_upd; pred_apply; cancel.
 
     rewrite <- diskIs_combine_upd with (m:=m); cancel.
-    admit.
+    rewrite map_add_cardinal; eauto.
+    intro Hm; destruct Hm as [? Hm]. apply Map.find_1 in Hm. congruence.
 
     destruct (weq a a0); subst.
     apply mapsto_add in H; subst.
@@ -224,9 +248,7 @@ Module BUFCACHE.
     apply pimpl_or_r. left. cancel.
     rewrite <- diskIs_combine_same with (m:=m); try pred_apply; cancel.
 
-    apply pimpl_or_r. left. cancel.
-    eauto.
-    eauto.
+    apply pimpl_or_r. left. cancel; eauto.
   Qed.
 
   Hint Extern 1 ({{_}} progseq (write _ _ _) _) => apply write_ok : prog.
@@ -234,7 +256,7 @@ Module BUFCACHE.
   Theorem sync_ok : forall a cs,
     {< d F v,
     PRE      rep cs d * [[ (F * a |-> v)%pred d ]]
-    POST:cs' exists d', rep cs' d' * [[ (F * a |-> (fst v, nil))%pred d' ]]
+    POST:cs  exists d', rep cs d' * [[ (F * a |-> (fst v, nil))%pred d' ]]
     CRASH    exists cs', rep cs' d \/
              exists d', rep cs' d' * [[ (F * a |-> (fst v, nil))%pred d' ]]
     >} sync a cs.
@@ -259,13 +281,15 @@ Module BUFCACHE.
     rewrite <- diskIs_combine_same with (m:=m); try pred_apply; cancel.
     eauto.
     eauto.
+    eauto.
+    eauto.
   Qed.
 
   Hint Extern 1 ({{_}} progseq (sync _ _) _) => apply sync_ok : prog.
 
   Theorem init_ok : forall cachesize,
     {< F,
-    PRE      F
+    PRE      F * [[ cachesize <> 0 ]]
     POST:cs  exists d, rep cs d * [[ F d ]]
     CRASH    F
     >} init cachesize.
@@ -287,7 +311,10 @@ Module BUFCACHE.
     apply sep_star_lift_apply'; eauto.
     apply sep_star_lift_apply'; eauto.
     apply sep_star_lift_apply'; eauto.
+    apply sep_star_lift_apply'; eauto.
+    apply sep_star_lift_apply'; eauto.
     congruence.
+    omega.
     intros.
     contradict H0; apply Map.empty_1.
   Qed.
@@ -387,12 +414,15 @@ Module BUFCACHE.
     rewrite crash_xform_diskIs.
     repeat rewrite crash_xform_lift_empty.
     cancel.
-    instantiate (a0 := (Map.empty valu, $0)).
+    instantiate (a0 := Build_cachestate (Map.empty valu) 0 (CSMaxCount cs) (CSEvict cs)).
     auto.
+    simpl; omega.
+    simpl in *; omega.
     inversion H.
   Qed.
 
   Hint Extern 0 (okToUnify (rep _ _) (rep _ _)) => constructor : okToUnify.
+
 End BUFCACHE.
 
 Global Opaque BUFCACHE.init.
